FreydSSA/Ctx/Var/Perm.lean
@@ -1,0 +1,45 @@
+import FreydSSA.Ctx.Var
+
+inductive Ctx.TPerm : Ctx ν α → Ctx ν α → Prop
+  | nil : TPerm [] []
+  | cons : TPerm Γ Δ → TPerm (⟨n, a⟩::Γ) (⟨n, a⟩::Δ)
+  | swap (v v' Γ) : v.name ≠ v'.name -> TPerm (v::v'::Γ) (v'::v::Γ)
+  | trans : TPerm Γ Δ → TPerm Δ Ξ → TPerm Γ Ξ
+
+theorem Ctx.TPerm.perm {Γ Δ : Ctx ν α} (h : Γ.TPerm Δ) : Γ.Perm Δ := by
+  induction h <;> constructor <;> assumption
+
+theorem Ctx.TPerm.refl {Γ : Ctx ν α} : Γ.TPerm Γ := by
+  induction Γ with
+  | nil => exact TPerm.nil
+  | cons v Γ I => exact TPerm.cons I
+
+theorem Ctx.TPerm.symm {Γ Δ : Ctx ν α} (h : Γ.TPerm Δ) : Δ.TPerm Γ := by
+  induction h with
+  | swap _ _ _ h => exact swap _ _ _ h.symm
+  | trans _ _ Il Ir => exact trans Ir Il
+  | _ => constructor <;> assumption
+
+-- theorem Ctx.TPerm.tail {Γ Δ : Ctx ν α} (h : TPerm Γ Δ) (h' : Γ.head? = Δ.head?)
+--   : TPerm Γ.tail Δ.tail := by
+--   induction Γ generalizing Δ with
+--   | nil => induction Δ with
+--     | nil => exact TPerm.nil
+--     | cons => cases h'
+--   | cons v Γ I => sorry
+
+-- theorem Ctx.TPerm.uncons {v : Var ν α} {Γ Δ : Ctx ν α} (h : TPerm (v::Γ) (v::Δ))
+--   : TPerm Γ Δ := h.tail rfl
+
+-- theorem Ctx.TPerm.comp {Γ Δ : Ctx ν α} (h : Γ.TPerm Δ) (h' : Γ.Comp Δ) : Γ = Δ := by
+--   cases h' with | mk base wl wr =>
+--   induction wl generalizing Δ with
+--   | nil => cases wr; rfl
+--   | cons vl wl I => cases wr with
+--     | cons _ wr =>
+--       cases I h.uncons wr
+--       rfl
+--     | skip hvr wr => sorry -- contradiction by perm...
+--   | skip hvl wl I => cases wr with
+--     | cons vr wr => sorry -- contradiction by perm...
+--     | skip hvr wr => exact I h wr
